library/init/data/bool/lemmas.lean
@@ -47,22 +47,22 @@ by cases b; simp
 @[simp] lemma bxor_tt (b : bool) : bxor b tt = bnot b :=
 by cases b; simp
 
-@[simp] lemma bxor_ff (b : bool) : bxor b ff = b :=
+lemma bxor_ff (b : bool) : bxor b ff = b :=
 by cases b; simp
 
 @[simp] lemma tt_bxor (b : bool) : bxor tt b = bnot b :=
 by cases b; simp
 
-@[simp] lemma ff_bxor (b : bool) : bxor ff b = b :=
+lemma ff_bxor (b : bool) : bxor ff b = b :=
 by cases b; simp
 
 @[simp] lemma bnot_bnot (b : bool) : bnot (bnot b) = b :=
 by cases b; simp
 
-@[simp] lemma tt_eq_ff_eq_false : ¬(tt = ff) :=
+lemma tt_eq_ff_eq_false : ¬(tt = ff) :=
 by contradiction
 
-@[simp] lemma ff_eq_tt_eq_false : ¬(ff = tt) :=
+lemma ff_eq_tt_eq_false : ¬(ff = tt) :=
 by contradiction
 
 @[simp] lemma eq_ff_eq_not_eq_tt (b : bool) : (¬(b = tt)) = (b = ff) :=
@@ -101,10 +101,10 @@ show (ff = tt) = false, by simp
 @[simp] lemma coe_tt : ↑tt = true :=
 show (tt = tt) = true, by simp
 
-@[simp] lemma coe_sort_ff : ↥ff = false :=
+lemma coe_sort_ff : ↥ff = false :=
 show (ff = tt) = false, by simp
 
-@[simp] lemma coe_sort_tt : ↥tt = true :=
+lemma coe_sort_tt : ↥tt = true :=
 show (tt = tt) = true, by simp
 
 @[simp] theorem to_bool_iff (p : Prop) [d : decidable p] : (to_bool p = tt) ↔ p :=
